# Algebraic Expressions Review

## Simplify each of the following rational expressions. Leave answers in factored form.

1. `((x^2 - 9x + 8) / (3x^2 - 24x)) * ((4x^3) / (x^2 - 1))`
> ```rs
> = (x^2 - 9x + 8)(4x^3) / (3x^2 - 24x)(x^2 - 1)
> = (x^2 - 9x + 8)(4x^3) / 3x(x - 8)(x^2 - 1)
> = (x - 1)(x - 8)(4x^3) / 3x(x - 8)(x^2 - 1)
> = (x - 1)(x - 8)(4x^3) / 3x(x - 8)(x + 1)(x - 1)
> = 4x^3 / 3x(x + 1)
> ```

2. `(((x^3) - 64) / (7x - 28)) * (42 / (3x^2 + 12x + 48))`
> ```rs
> // Difference of cubes: a³ − b³ = (a − b)(a² + ab + b²)
> = ((x - 4)(x^2 + 4x + 16) / (7x - 28)) * (42 / (3x^2 + 12x + 48))
> = 42(x - 4)(x^2 + 4x + 16) / (7x - 28)(3x^2 + 12x + 48)
> = 42(x - 4)(x^2 + 4x + 16) / 3(7x - 28)(x^2 + 4x + 16)
> = 42(x - 4) / 3(7x - 28)
> = 42(x - 4) / 21(x - 4)
> = 42 / 21
> = 2
> ```

3. `((x^2 - 9x - 22) / (x^2 + 5x - 24)) / ((x + 2) / (x - 3))`
> ```rs
> = ((x^2 - 9x - 22) / (x^2 + 5x - 24)) * ((x - 3) / (x + 2))
> = ((x - 3)(x^2 - 9x - 22)) / ((x + 2)(x^2 + 5x - 24))
> = ((x - 3)(x^2 - 9x - 22)) / ((x + 2)(x + 8)(x - 3))
> = ((x - 3)(x + 2)(x - 11)) / ((x + 2)(x + 8)(x - 3))
> = (x - 11) / (x + 8)
> ```

4. `((x^4 - 13x^2 + 36) / (x^4 - 14x^2 - 32)) / ((x^3 + 3x^2 - 4x - 12) / (x^3 - 4x^2 + 2x - 8))`
> ```rs
> = ((x^4 - 13x^2 + 36) / (x^4 - 14x^2 - 32)) * ((x^3 - 4x^2 + 2x - 8) / (x^3 + 3x^2 - 4x - 12))
> = ((x^4 - 13x^2 + 36)(x^3 - 4x^2 + 2x - 8) / (x^4 - 14x^2 - 32)(x^3 + 3x^2 - 4x - 12))
> = ((x^4 - 13x^2 + 36)(x^2(x - 4) + 2(x - 4))) / ((x^4 - 14x^2 - 32)(x^3 + 3x^2 - 4x - 12))
> = ((x^4 - 13x^2 + 36)(x^2 + 2)(x - 4)) / ((x^4 - 14x^2 - 32)(x^3 + 3x^2 - 4x - 12))
> = ((x^4 - 13x^2 + 36)(x^2 + 2)(x - 4)) / ((x^4 - 14x^2 - 32)(x^2(x + 3) - 4(x + 3)))
> = ((x^4 - 13x^2 + 36)(x^2 + 2)(x - 4)) / ((x^4 - 14x^2 - 32)((x^2 - 4)(x + 3)))
> = ((x^4 - 13x^2 + 36)(x^2 + 2)(x - 4)) / ((x^4 - 14x^2 - 32)((x + 2)(x - 2)(x + 3)))
> = ((x^4 - 13x^2 + 36)(x^2 + 2)(x - 4)) / ((x^2 + 2)(x + 4)(x - 4)(x + 2)(x - 2)(x + 3))
> = ((x^2 - 4)(x^2 - 9)(x^2 + 2)(x - 4)) / ((x^2 + 2)(x + 4)(x - 4)(x + 2)(x - 2)(x + 3))
> = ((x + 2)(x - 2)(x + 3)(x - 3)(x^2 + 2)(x - 4)) / ((x^2 + 2)(x + 4)(x - 4)(x + 2)(x - 2)(x + 3))
> // Cancel out the terms (x - 2), (x + 2), (x + 3), (x^2 + 2), and (x - 4)
> = (x - 3) / (x + 4)
> ```

4. `((x^4 - 13x^2 + 36) / (x^4 - 14x^2 - 32)) / ((x^3 + 3x^2 - 4x - 12) / (x^3 - 4x^2 + 2x - 8))`
> ```rs
> = ((x^4 - 13x^2 + 36) / (x^4 - 14x^2 - 32)) * ((x^3 - 4x^2 + 2x - 8) / (x^3 + 3x^2 - 4x - 12))
> = ((x^4 - 13x^2 + 36)(x^3 - 4x^2 + 2x - 8) / (x^4 - 14x^2 - 32)(x^3 + 3x^2 - 4x - 12))
> = ((x^4 - 13x^2 + 36)(x^2(x - 4) + 2(x - 4))) / ((x^4 - 14x^2 - 32)(x^3 + 3x^2 - 4x - 12))
> = ((x^4 - 13x^2 + 36)(x^2 + 2)(x - 4)) / ((x^4 - 14x^2 - 32)(x^3 + 3x^2 - 4x - 12))
> = ((x^4 - 13x^2 + 36)(x^2 + 2)(x - 4)) / ((x^4 - 14x^2 - 32)(x^2(x + 3) - 4(x + 3)))
> = ((x^4 - 13x^2 + 36)(x^2 + 2)(x - 4)) / ((x^4 - 14x^2 - 32)((x^2 - 4)(x + 3)))
> = ((x^4 - 13x^2 + 36)(x^2 + 2)(x - 4)) / ((x^4 - 14x^2 - 32)((x + 2)(x - 2)(x + 3)))
> = ((x^4 - 13x^2 + 36)(x^2 + 2)(x - 4)) / ((x^2 + 2)(x + 4)(x - 4)(x + 2)(x - 2)(x + 3))
> = ((x^2 - 4)(x^2 - 9)(x^2 + 2)(x - 4)) / ((x^2 + 2)(x + 4)(x - 4)(x + 2)(x - 2)(x + 3))
> = ((x + 2)(x - 2)(x + 3)(x - 3)(x^2 + 2)(x - 4)) / ((x^2 + 2)(x + 4)(x - 4)(x + 2)(x - 2)(x + 3))
> // Cancel out the terms (x - 2), (x + 2), (x + 3), (x^2 + 2), and (x - 4)
> = (x - 3) / (x + 4)
> ```

5. `(1 / x) + (1 / y)`
> ```rs
> = (y / xy) + (x / xy)
> = (y + x) / xy
> ```

6. `(5 / 2xy) - (2 / 7y)`
> ```rs
> = (35xy / 14) - (4y / 14)
> = (35xy - 4y) / 14
> = y(35x - 4) / 14
> ```

7. `((x + 2) / (x - 1)) - (2 / (x + 6)) - (14 / (x^2 + 5x - 6))`
> ```rs
> = ((x + 2) / (x - 1)) - (2 / (x + 6)) - (14 / (x - 1)(x + 6))
> = ((x + 2)(x + 6) / (x - 1)(x + 6)) - (2(x - 1) / (x + 6)(x - 1)) - (14 / (x - 1)(x + 6))
> = ((x + 2)(x + 6) - 2(x - 1) - 14) / (x - 1)(x + 6)
> = ((x^2 + 8x + 12) - 2(x - 1) - 14) / (x - 1)(x + 6)
> = ((x^2 + 8x + 12) - 2x + 2 - 14) / (x - 1)(x + 6)
> = (x^2 + 6x) / (x - 1)(x + 6)
> = x(x + 6) / (x - 1)(x + 6)
> = x / (x - 1)
> ```

8. `((x - 5) / (x^2 - 3x)) + (5 / (2x^2))`
> ```rs
> = ((x - 5) / x(x - 3)) + (5 / (2x^2))
> = (2x(x - 5) / 2x^2(x - 3)) + (5(x - 3) / 2x^2(x - 3))
> = ((2x(x - 5) + 5(x - 3)) / 2x^2(x - 3))
> = (2x^2 - 10x + 5x - 15) / 2x^2(x - 3)
> = (2x^2 - 5x - 15) / 2x^2(x - 3)
> ```

9. `((x - 3) / (x^2 - 2x - 3)) + (3 / (x^2 + 3x + 2))`
> ```rs
> = ((x - 3) / (x + 1)(x - 3)) + (3 / (x^2 + 3x + 2))
> = ((x - 3) / (x + 1)(x - 3)) + (3 / (x + 1)(x + 2))
> = (1 / (x + 1)) + (3 / (x + 1)(x + 2))
> = ((x + 2) / (x + 1)(x + 2)) + (3 / (x + 1)(x + 2))
> = (x + 2 + 3) / (x + 1)(x + 2)
> = (x + 5) / (x + 1)(x + 2)
> ```

10. `(6 / (x^2 - 3x)) + (2 / (3 - x))`
> ```rs
> = (6 / x(x - 3)) + (2 / (3 - x))
> = (6 / x(x - 3)) - (2 / (x - 3))
> = (6 / x(x - 3)) - (2x / x(x - 3))
> = (6 - 2x) / x(x - 3)
> = -2(x - 3) / x(x - 3)
> = -2 / x
> ```

11. `(3 / 2x) + 6`
> ```rs
> = (3 / 2x) + (12 / 2)
> = (3x + 12) / 2
> = 3(x + 4) / 2
> ```

12. `((x / 4) - (4 / x)) / (1 - (4 / x))`
> ```rs
> = ((x^2 / 4x) - (16 / 4x)) / ((x / x) - (4 / x))
> = ((x^2 - 16) / 4x) / ((x - 4) / x)
> = ((x + 4)(x - 4) / 4x) / ((x - 4) / x)
> = x(x + 4)(x - 4) / 4x(x - 4)
> = (x + 4) / 4
> ```

13. `((x / (x + 3)) - (2 / (x + 1))) / (((3x + 5) / (x^2 + 4x + 3)) - (1 / (x + 3)))`
> ```rs
> = ((x / (x + 3)) - (2 / (x + 1))) / (((3x + 5) / (x + 3)(x + 1)) - (1 / (x + 3)))
> = ((x / (x + 3)) - (2 / (x + 1))) / (((3x + 5) / (x + 3)(x + 1)) - ((-x - 1) / (x + 3)(x + 1)))
> = ((x / (x + 3)) - (2 / (x + 1))) / ((3x + 5 - x - 1) / (x + 3)(x + 1))
> = ((x / (x + 3)) - (2 / (x + 1))) / ((2x + 4) / (x + 3)(x + 1))
> = ((x / (x + 3)) - (2 / (x + 1))) / (2(x + 2) / (x + 3)(x + 1))
> = ((x(x + 1) / (x + 1)(x + 3)) - (2(x + 3) / (x + 1)(x + 3))) / (2(x + 2) / (x + 3)(x + 1))
> = ((x(x + 1) - 2(x + 3)) / (x + 1)(x + 3)) / (2(x + 2) / (x + 3)(x + 1))
> = ((x^2 + x - 2x - 6) / (x + 1)(x + 3)) / (2(x + 2) / (x + 3)(x + 1))
> = ((x^2 - x - 6) / (x + 1)(x + 3)) / (2(x + 2) / (x + 3)(x + 1))
> = ((x + 2)(x - 3) / (x + 1)(x + 3)) / (2(x + 2) / (x + 3)(x + 1))
> = (x + 2)(x - 3)(x + 3)(x + 1) / 2(x + 2)(x + 1)(x + 3)
> = (x - 3) / 2
> ```

14. `((4 / (x - 5)) + (5 / (x - 5))) / ((2 / x) + (3 / (x - 5)))`
> ```rs
> = (9 / (x - 5)) / ((2 / x) + (3 / (x - 5)))
> = 9 / ((2 / x)(x - 5) + (3 / (x - 5))(x - 5))
> = 9 / ((2 / x)(x - 5) + 3)
> = 9 / ((2(x - 5) / x) + 3)
> = 9 / (((2x - 10) / x) + 3)
> = 9 / (((2x - 10) + 3x / x))
> = 9 / ((5x - 10) / x)
> = 9 / (5(x - 2) / x)
> = 9x / 5(x - 2)
> ```

15. `((2 / y^2) - (5 / xy) - (3 / x^2)) / ((2 / y^2) + (7 / xy) + (3 / x^2))`
> ```rs
> = ((2 / y^2) - (5 / xy) - (3 / x^2)) / ((2x^2 / x^2y^2) + (7xy / x^2y^2) + (3y^2 / x^2y^2))
> = ((2 / y^2) - (5 / xy) - (3 / x^2)) / ((2x^2 + 7xy + 3y^2) / x^2y^2)
> = ((2 / y^2) - (5 / xy) - (3 / x^2)) / ((x(y + 2x) + 3y(y + 2x)) / x^2y^2)
> = ((2 / y^2) - (5 / xy) - (3 / x^2)) / (((x + 3y)(y + 2x)) / x^2y^2)
> = ((2x^2 / x^2y^2) - (5xy / x^2y^2) - (3y^2 / x^2y^2)) / (((x + 3y)(y + 2x)) / x^2y^2)
> = ((2x^2 - 5xy - 3y^2) / x^2y^2) / (((x + 3y)(y + 2x)) / x^2y^2)
> = ((x(y + 2x) - 3y(y + 2x)) / x^2y^2) / (((x + 3y)(y + 2x)) / x^2y^2)
> = ((x - 3y)(y + 2x) / x^2y^2) / ((x + 3y)(y + 2x) / x^2y^2)
> = (x - 3y)(y + 2x)(x^2y^2) / (x + 3y)(y + 2x)(x^2y^2)
> = (x - 3y) / (x + 3y)
> ```