# Equation Review

## Solve the following equations.

1. $2x - (1 - x) = 11 - x$
> $= 3x - 1 = 11 - x$
> 
> $= 4x = 12$
> 
> $= x = 3$
2. $\frac{2}{5}(x - 2) = \frac{1}{4}(x) + 4$
> $= \frac{2(x - 2)}{5} = \frac{x}{4} + 4$
>
> $= \frac{2(x - 2)}{5} = \frac{x}{4} + \frac{16}{4}$
>
> $= \frac{2(x - 2)}{5} = \frac{x + 16}{4}$
>
> $= \frac{8(x - 2)}{20} = \frac{5(x + 16)}{20}$
>
> $= 8(x - 2) = 5(x + 16)$
>
> $= 8x - 16 = 5x + 80$
>
> $= 3x = 96$
>
> $= x = 3$
3. $x^2 + 3x = 10$
> $= x^2 + 3x - 10 = 0$
> 
> Factors of $-10$ that add to $3$ are $\lbrace 5, -2 \rbrace$<br>
> $= (x + 5)(x - 2) = 0$
> 
> Split factors<br>
> $= x = \lbrace -5, 2 \rbrace$
4. $x^4 - 40x^2 + 144 = 0$
> Let $y = x^2$<br>
> $= y^2 - 40y + 144 = 0$
> 
> Factors of $144$ that add to $-40$ are $\lbrace -4, -36 \rbrace$<br>
> $= (y - 4)(y - 36) = 0$
> 
> $= (x^2 - 4)(x^2 - 36) = 0$
> 
> Difference of squares: $a^2 - b^2 = (a + b)(a - b)$<br>
> $= (x + 2)(x - 2)(x + 6)(x - 6) = 0$
> 
> Split factors<br>
> $= x = \lbrace 2, -2, 6, -6 \rbrace$
5. $x^2 - 20 = 0$
> $= x^2 = 20$
> 
> $= x = \pm \sqrt{20}$
> 
> $= x = \pm 2\sqrt{5}$
6. $4x^3 - 19x^2 - 5x = 0$
> $= x(4x^2 - 19x - 5) = 0$
> 
> Factors of $-20$ that add up to $-19$ are $\lbrace -20, 1 \rbrace$<br>
> $= x(4x^2 + x - 20x - 5)$
> 
> $= x(x(4x + 1) - 5(4x + 1))$
> 
> $= x(x - 5)(4x + 1)$
> 
> Split factors<br>
> $= x = \lbrace 0, 5, 1 / 4 \rbrace$
7. $x^3 - 2x^2 - 4x + 8 = 0$
> $= (xÂ³ - 2x^2) + (-4x + 8) = 0$
> 
> $= x^2(x - 2) - 4(x - 2) = 0$
> 
> $= (x^2 - 4)(x - 2) = 0$
> 
> Difference of squares: $a^2 - b^2 = (a + b)(a - b)$<br>
> $= (x + 2)(x - 2)(x - 2) = 0$
> 
> Split roots<br>
> $= x = \lbrace +2, -2 \rbrace$
8. $4x^2 = 60x$
> Divide by $4x$<br>
> $= x = 15$
9. $(x - 5)(x - 6) = x(x + 3) + 7$
> Expand terms<br>
> $= x^2 - 6x - 5x + 30 = x^2 + 3x + 7$
> 
> $= x^2 - 11x + 30 = x^2 + 3x + 7$
>
> $= -11x + 30 = 3x + 7$
>
> $= -14x + 30 = 7$
>
> $= -14x = -23$
>
> $= x = +23 / 14$
10. $5x^2 + 7x + 20 = 7x^2 + 3x - 10$
> $= 5x^2 + 7x + 20 - 7x^2 - 3x + 10 = 0$
> 
> Combine terms<br>
> $= -2x^2 + 4x + 30 = 0$
> 
> $= -2(x^2 - 2x - 15) = 0$
> 
> Factors of $-15$ that add up to $-2$ are $\lbrace 3, -5 \rbrace$<br>
> $= -2(x + 3)(x - 5) = 0$
> 
> Split factors<br>
> $= x = \lbrace -3, +5 \rbrace$
11. $x^2 + 8x - 4 = 0$
> Add $20$ to both sides
> $= x^2 + 8x + 16 = 20$
> 
> Factors of $16$ that add to $8$ are $\lbrace 4, 4 \rbrace$<br>
> $= (x + 4)(x + 4) = 20$
> 
> $= (x + 4)^2 = 20$
> 
> $= x + 4 = \pm \sqrt{20}$
> 
> $= x = \pm \sqrt{20} - 4$
> 
> $= x = \pm (2\sqrt{5}) - 4$
12. $x(x - 4) = 12$
> $= x^2 - 4x = 12$
> 
> $= x^2 - 4x - 12 = 0$
> 
> Factors of $-12$ that add up to $-4$ are $\lbrace -6, 2 \rbrace$<br>
> $= (x - 6)(x + 2) = 0$
> 
> Split factors<br>
> $= x = \lbrace +6, -2 \rbrace$
13. $2x^2 - 50 = 0$
> $= 2(x^2 - 25) = 0$
> 
> Difference of squares: $a^2 - b^2 = (a + b)(a - b)$<br>
> $= 2(x + 5)(x - 5) = 0$
> 
> Split factors<br>
> $= x = \lbrace +5, -5 \rbrace$
14. $6x^2 + x = 2$
> $6x^2 + x - 2 = 0$
>
> Factors of $-12$ that add up to $1$ are $\lbrace -3, 4 \rbrace$
>
> $6x^2 - 3x + 4x - 2 = 0$
>
> $3x(2x - 1) + 2(2x - 1) = 0$
>
> $(3x + 2)(2x - 1) = 0$
>
> Split factors<br>
> $x = \lbrace \frac{2}{3}, -\frac{1}{2} \rbrace$

## Solve each equation for the indicated variable.

15. $y = mx + b$ for $m$
> $= y - b = mx$
> 
> $= (y - b) / x = m$
16. $5cy - d = 4d - cy$ for $y$
> $= 5cy - d - 4d + cy = 0$
>
> $= 6cy - 5d = 0$
>
> $= 6cy = 5d$
>
> $= y = 5d / 6c$
17. $V = \frac{1}{3}(bwh)$ for `h`
> $= 3V = bwh$
> 
> $= \frac{3V}{bw} = h$
18. $A = p(1 + rt)$ for $r$
> $= A / p = 1 + rt$
> 
> $= A / p - 1 = rt$
> 
> $= (A / p - 1) / t = r$
19. $a(2 + b) = 6b - 5$ for $b$
> $= 2a + ab - 6b + 5 = 0$
>
> $= 2a + b(a - 6) + 5 = 0$
>
> $= b(a - 6) = -5 - 2a$
>
> $= b = (-5 - 2a) / (a - 6)$

20. $ax^2 + bx = 0$ for $x$
> $= x(ax + b) = 0$
>
> $= ax + b = 0 / x$
>
> $= ax + b = 0$
>
> $= ax = -b$
>
> $= x = -b / a$