# Factoring Review

## Multiply each of the following polynomials.
1. $(2x + 3)(x - 1)$
> $= 2x^2 - 2x + 3x - 3$
> 
> $= 2x^2 + x - 3$
2. $(x + 3)$
> $= (x + 3)(x + 3)$
>
> $= x^2 + 3x + 3x + 9$
>
> $= x^2 + 6x + 9$
3. $(2x - 1)$
> $= (2x - 1)(2x - 1)$
>
> $= 2x^2 - 2x - 2x + 1$ 
> 
> $= 2x^2 - 4x + 1$
4. $(x^2 + 3x + 2)(2x - 1)$
> $= (2x^3 + 6x^2 + 4x) + (-x^2 - 3x - 2)$
> 
> $= 2x^3 + 5x^2 + x - 2$


## Factor each polynomial completely.
5. $x^2 + 10x + 9$
> $= (x + 9)(x + 1)$
6. $3x^2 - 3y^2$
> $= 3(x^2 - y^2)$
> 
> Difference of squares: $a^2 - b^2 = (a + b)(a - b)$
> 
> $= 3(x + y)(x - y)$
7. $12x^3 - 34x^2 + 10x$
> $= 2x(6x^2 - 17x + 5)$
>
> $= 2x(6x^2 - 15x - 2x + 5)$
>
> $= 2x(2x(3x - 1) - 5(3x - 1))$
>
> $= 2x(2x - 5)(3x - 1)$

8. $6x^2 + 13x + 6$
> $= 6x^2 + 9x + 4x + 6$
>
> $= 3(3x + 2) + 2x(3x + 2)$
>
> $= (3 + 2x)(3x + 2)$

9. $-3xy^2 + 9x$
> $= -3x(y^2 - 3)$
10. $x^2 + 8xy + 16y^2$
> $= (4y + x)(4y + x)$
> 
> $= (4y + x)^2$
11. $6x^2 + 27x - 15$
> $= 3(2x^2 + 9x - 5)$
>
> $= 3(2x^2 + 10x - x - 5)$
>
> $= 3(5(2x - 1) + x(2x - 1))$
>
> $= 3(5 + x)(2x - 1)$

12. $x^4 - 16$
> Difference of squares: $a^2 - b^2 = (a + b)(a - b)$
> 
> $= (x^2 + 4)(x^2 - 4)$
> 
> $= (x^2 + 4)(x + 2)(x - 2)$
13. $10x^3y - 12x^2y^2$
> $= 2x^2y(-6y + 5x)$
14. $x^2 - 12x + 20$
> $= (x - 2)(x - 10)$
15. $36 - x^2$
> Difference of squares: $a^2 - b^2 = (a + b)(a - b)$
> 
> $= (6 + x)(6 - x)$

16. $5x^2 + 15x - 10$
> $= 5(x^2 + 3x - 2)$
17. $3x^2 + 24x + 45$
> $= 3(x^2 + 8x + 15)$
> 
> $= 3(x + 5)(x + 3)$
18. $81y^2 - 49$
> $= (9y)^2 - 7^2$
> 
> Difference of squares: $a^2 - b^2 = (a + b)(a - b)$
> 
> $= (9y + 7)(9y - 7)$
19. $49x^2 + 14x + 1$
> $= 49x^2 + 7x + 7x + 1$
> 
> $= (7x + 1) + 7x(7x + 1)$
> 
> $= (7x + 1)(7x + 1)$
> 
> $= (7x + 1)^2$
20. $x^3 + 3x^2 + 2x + 6$
> = $(x^3 + 3x^2) + (2x + 6)$
> 
> = $x^2(x + 3) + 2(x + 3)$
> 
> = $(x^2 + 2)(x + 3)$
21. $x^4 + 27x$
> $= x(x^3 + 27)$
> 
> Sum of cubes: $a^3 + b^3 = (a + b)(a^2 - ab + b^2)$
> 
> $= x(x + 3)(x^2 - 3x + 9)$

22. $x^4 - x^3 + x - 1$
> $= (x^4 - x^3) + (x - 1)$
> 
> $= x^3(x - 1) + (x - 1)$
> 
> $= (x^3 + 1)(x - 1)$
> 
> Sum of cubes: $a^3 + b^3 = (a + b)(a^2 - ab + b^2)$
> 
> $= (x^2 - x + 1)(x + 1)(x - 1)$
23. $x^3 - 3x^2 - x + 3$
> $= (x^3 - 3x^2) - (x - 3)$
>
> $= x^2(x - 3) - (x - 3)$
>
> $= (x^2 - 1)(x - 3)$
>
> Difference of squares: $a^2 - b^2 = (a + b)(a - b)$
> 
> $= (x + 1)(x - 1)(x - 3)$
24. $x^6 - 64$
> Difference of squares: $a^2 - b^2 = (a + b)(a - b)$
> 
> $= (x^3 + 8)(x^3 - 8)$
> Sum of cubes: $a^3 + b^3 = (a + b)(a^2 - ab + b^2)$
> 
> Difference of cubes: $a^3 − b^3 = (a − b)(a^2 + ab + b^2)$
> 
> $= (x + 2)(x^2 - 2x + 4)(x - 2)(x^2 + 2x + 4)$

25. $3x^2 - 27y^2$
> $= 3(x^2 - 9y^2)$
> 
> $= 3(x^2 - (3y)^2)$
> 
> Difference of squares: $a^2 - b^2 = (a + b)(a - b)$
> 
> $= 3(x + 3y)(x - 3y)$
