# Algebraic Expressions Review

## Simplify each of the following rational expressions. Leave answers in factored form.

1. $\frac{(x^2 - 9x + 8)}{(3x^2 - 24x)} * \frac{4x³}{x^2 - 1}$
> $= \frac{(x^2 - 9x + 8)(4x³)}{(3x^2 - 24x)(x^2 - 1)}$
>
> $= \frac{(x^2 - 9x + 8)(4x³)}{3x(x - 8)(x^2 - 1)}$
>
> $= \frac{(x - 1)(x - 8)(4x³)}{3x(x - 8)(x^2 - 1)}$
>
> $= \frac{(x - 1)(x - 8)(4x³)}{3x(x - 8)(x + 1)(x - 1)}$
>
> $= \frac{4x³}{3x(x + 1)}$


2. $\frac{x³ - 64}{7x - 28} * \frac{42}{3x^2 + 12x + 48}$
> Difference of cubes: $a³ − b³ = (a − b)(a^2 + ab + b^2)$
> 
> $= \frac{(x - 4)(x^2 + 4x + 16)}{(7x - 28)} * \frac{42}{3x^2 + 12x + 48}$
>
> $= \frac{42(x - 4)(x^2 + 4x + 16)}{(7x - 28)(3x^2 + 12x + 48)}$
>
> $= \frac{42(x - 4)(x^2 + 4x + 16)}{3(7x - 28)(x^2 + 4x + 16)}$
>
> $= \frac{42(x - 4)}{3(7x - 28)}$
>
> $= \frac{42(x - 4)}{21(x - 4)}$
>
> $= \frac{42}{21}$
>
> $= 2$

3. $\frac{\frac{x^2 - 9x - 22}{x^2 + 5x - 24}}{\frac{x + 2}{x - 3}}$
> $= \frac{x^2 - 9x - 22}{x^2 + 5x - 24} * \frac{x - 3}{x + 2}$
>
> $= \frac{(x - 3)(x^2 - 9x - 22)}{(x + 2)(x^2 + 5x - 24)}$
>
> $= \frac{(x - 3)(x^2 - 9x - 22)}{(x + 2)(x + 8)(x - 3)}$
>
> $= \frac{(x - 3)(x + 2)(x - 11)}{(x + 2)(x + 8)(x - 3)}$
>
> $= \frac{x - 11}{x + 8}$


4. $\frac{\frac{x⁴ - 13x^2 + 36}{x⁴ - 14x^2 - 32}}{\frac{x³ + 3x^2 - 4x - 12}{x³ - 4x^2 + 2x - 8}}$
> $= \frac{x⁴ - 13x^2 + 36}{x⁴ - 14x^2 - 32} * \frac{x³ - 4x^2 + 2x - 8}{x³ + 3x^2 - 4x - 12}$
>
> $= \frac{(x⁴ - 13x^2 + 36)(x³ - 4x^2 + 2x - 8)}{(x⁴ - 14x^2 - 32)(x³ + 3x^2 - 4x - 12)}$
>
> $= \frac{(x⁴ - 13x^2 + 36)(x^2(x - 4) + 2(x - 4))}{(x⁴ - 14x^2 - 32)(x³ + 3x^2 - 4x - 12)}$
>
> $= \frac{(x⁴ - 13x^2 + 36)(x^2 + 2)(x - 4)}{(x⁴ - 14x^2 - 32)(x³ + 3x^2 - 4x - 12)}$
>
> $= \frac{(x⁴ - 13x^2 + 36)(x^2 + 2)(x - 4)}{(x⁴ - 14x^2 - 32)(x^2(x + 3) - 4(x + 3))}$
>
> $= \frac{(x⁴ - 13x^2 + 36)(x^2 + 2)(x - 4)}{(x⁴ - 14x^2 - 32)(x^2 - 4)(x + 3)}$
>
> $= \frac{(x⁴ - 13x^2 + 36)(x^2 + 2)(x - 4)}{(x⁴ - 14x^2 - 32)(x + 2)(x - 2)(x + 3)}$
>
> $= \frac{(x⁴ - 13x^2 + 36)(x^2 + 2)(x - 4)}{(x^2 + 2)(x + 4)(x - 4)(x + 2)(x - 2)(x + 3)}$
>
> $= \frac{(x^2 - 4)(x^2 - 9)(x^2 + 2)(x - 4)}{(x^2 + 2)(x + 4)(x - 4)(x + 2)(x - 2)(x + 3)}$
>
> $= \frac{(x + 2)(x - 2)(x + 3)(x - 3)(x^2 + 2)(x - 4)}{(x^2 + 2)(x + 4)(x - 4)(x + 2)(x - 2)(x + 3)}$
>
> Cancel out the terms $(x - 2)$, $(x + 2)$, $(x + 3)$, $(x^2 + 2)$, and $(x - 4)$
> 
> = $\frac{x - 3}{x + 4}$

5. $\frac{1}{x} + \frac{1}{y}$
> $= \frac{y}{xy} + \frac{x}{xy}$
> 
> $= \frac{y + x}{xy}$

6. $\frac{5}{2xy} - \frac{2}{7y}$
> $= \frac{35xy}{14} - \frac{4y}{14}$
>
> $= \frac{35xy - 4y}{14}$
>
> $= \frac{y(35x - 4)}{14}$


7. $\frac{x + 2}{x - 1} - \frac{2}{x + 6} - \frac{14}{x^2 + 5x - 6}$
> $= \frac{x + 2}{x - 1} - \frac{2}{x + 6} - \frac{14}{(x - 1)(x + 6)}$
>
> $= \frac{(x + 2)(x + 6)}{(x - 1)(x + 6)} - \frac{2(x - 1)}{(x + 6)(x - 1)} - \frac{14}{(x - 1)(x + 6)}$
>
> $= \frac{(x + 2)(x + 6) - 2(x - 1) - 14}{(x - 1)(x + 6)}$
>
> $= \frac{(x^2 + 8x + 12) - 2(x - 1) - 14}{(x - 1)(x + 6)}$
>
> $= \frac{(x^2 + 8x + 12) - 2x + 2 - 14}{(x - 1)(x + 6)}$
>
> $= \frac{x^2 + 6x}{(x - 1)(x + 6)}$
>
> $= \frac{x(x + 6)}{(x - 1)(x + 6)}$
>
> $= \frac{x}{x - 1}$

8. $\frac{x - 5}{x^2 - 3x} + \frac{5}{2x^2}$
> $= \frac{x - 5}{x(x - 3)} + \frac{5}{2x^2}$
>
> $= \frac{2x(x - 5)}{2x^2(x - 3)} + \frac{5(x - 3)}{2x^2(x - 3)}$
>
> $= \frac{2x(x - 5) + 5(x - 3)}{2x^2(x - 3)}$
>
> $= \frac{2x^2 - 10x + 5x - 15}{2x^2(x - 3)}$
>
> $= \frac{2x^2 - 5x - 15}{2x^2(x - 3)}$

9.  $\frac{x - 3}{x^2 - 2x - 3} + \frac{3}{x^2 + 3x + 2}$
> = $\frac{x - 3}{(x + 1)(x - 3)} + \frac{3}{x^2 + 3x + 2}$
> 
> $= \frac{x - 3}{(x + 1)(x - 3)} + \frac{3}{(x + 1)(x + 2)}$
>
> $= \frac{1}{x + 1} + \frac{3}{(x + 1)(x + 2)}$
>
> $= \frac{x + 2}{(x + 1)(x + 2)} + \frac{3}{(x + 1)(x + 2)}$
>
> $= \frac{x + 2 + 3}{(x + 1)(x + 2)}$
>
> $= \frac{x + 5}{(x + 1)(x + 2)}$

10. $\frac{6}{x^2 - 3x} + \frac{2}{3 - x}$
> $= \frac{6}{x(x - 3)} + \frac{2}{3 - x}$
>
> $= \frac{6}{x(x - 3)} - \frac{2}{x - 3}$
>
> $= \frac{6}{x(x - 3)} - \frac{2x}{x(x - 3)}$
>
> $= \frac{6 - 2x}{x(x - 3)}$
>
> $= \frac{-2(x - 3)}{x(x - 3)}$
>
> $= \frac{-2}{x}$

11. $\frac{3}{2x} + 6$
> $= \frac{3(4x + 1)}{2x}$

12. $\frac{\frac{x}{4} - \frac{4}{x}}{1 - \frac{4}{x}}$
> $= \frac{x^2}{4x} - \frac{\frac{16}{4x}}{\frac{x}{x} - \frac{4}{x}}$
>
> $= \frac{\frac{x^2 - 16}{4x}}{\frac{x - 4}{x}}$
>
> $= \frac{\frac{(x + 4)(x - 4)}{4x}}{\frac{x - 4}{x}}$
>
> $= \frac{x(x + 4)(x - 4)}{4x(x - 4)}$
>
> $= \frac{x + 4}{4}$

13. $\frac{\frac{x}{x + 3} - \frac{2}{x + 1}}{\frac{3x + 5}{x^2 + 4x + 3} - \frac{1}{x + 3}}$

> $= \frac{\frac{x}{x + 3} - \frac{2}{x + 1}}{\frac{3x + 5}{(x + 3)(x + 1)} - \frac{1}{x + 3}}$
> 
> $= \frac{\frac{x}{x + 3} - \frac{2}{x + 1}}{\frac{3x + 5}{(x + 3)(x + 1)} - \frac{(-x - 1)}{(x + 3)(x + 1)}}$
> 
> $= \frac{(\frac{x}{x + 3} - \frac{2}{x + 1})}{(\frac{3x + 5 - x - 1}{(x + 3)(x + 1)})}$
> 
> $= \frac{\frac{x}{x + 3} - \frac{2}{x + 1}}{\frac{2x + 4}{(x + 3)(x + 1)}}$
> 
> $= \frac{\frac{x}{x + 3} - \frac{2}{x + 1}}{\frac{2(x + 2)}{(x + 3)(x + 1)}}$
> 
> $= \frac{\frac{x(x + 1)}{(x + 1)(x + 3)} - \frac{2(x + 3)}{(x + 1)(x + 3)}}{\frac{2(x + 2)}{(x + 3)(x + 1)}}$
> 
> $= \frac{\frac{x(x + 1) - 2(x + 3)}{(x + 1)(x + 3)}}{\frac{2(x + 2)}{(x + 3)(x + 1)}}$
> 
> $= \frac{\frac{x^2 + x - 2x - 6}{(x + 1)(x + 3)}}{\frac{2(x + 2)}{(x + 3)(x + 1)}}$
> 
> $= \frac{\frac{x^2 - x - 6}{(x + 1)(x + 3)}}{\frac{2(x + 2)}{(x + 3)(x + 1)}}$
> 
> $= \frac{\frac{(x + 2)(x - 3)}{(x + 1)(x + 3)}}{\frac{2(x + 2)}{(x + 3)(x + 1)}}$
> 
> $= \frac{(x + 2)(x - 3)(x + 3)(x + 1)}{2(x + 2)(x + 1)(x + 3)}$
> 
> $= \frac{(x - 3)}{2}$

14. $\frac{\frac{4}{x - 5} + \frac{5}{x - 5}}{\frac{\frac{2}{x}}{\frac{3}{x - 5}}}$
> $= \frac{\frac{9}{x - 5}}{\frac{2}{x} + \frac{3}{x - 5}}$
>
> $= \frac{9}{\frac{2}{x}(x - 5) + \frac{3}{x - 5}(x - 5)}$
>
> $= \frac{9}{\frac{2}{x}(x - 5) + 3}$
>
> $= \frac{9}{\frac{2(x - 5)}{x} + 3}$
>
> $= \frac{9}{\frac{2x - 10}{x} + 3}$
>
> $= \frac{9}{\frac{2x - 10 + 3x}{x}}$
>
> $= \frac{9}{\frac{5x - 10}{x}}$
>
> $= \frac{9}{\frac{5(x - 2)}{x}}$
>
> $= \frac{9x}{5(x - 2)}$

15. $\frac{\frac{2}{y^2} - \frac{5}{xy} - \frac{3}{x^2}}{\frac{2}{y^2} + \frac{7}{xy} + \frac{3}{x^2}}$
> $= \frac{\frac{2}{y^2} - \frac{5}{xy} - \frac{3}{x^2}}{\frac{2x^2}{x^2y^2} + \frac{7xy}{x^2y^2} + \frac{3y^2}{x^2y^2}}$
>
> $= \frac{\frac{2}{y^2} - \frac{5}{xy} - \frac{3}{x^2}}{\frac{2x^2 + 7xy + 3y^2}{x^2y^2}}$
>
> $= \frac{\frac{2}{y^2} - \frac{5}{xy} - \frac{3}{x^2}}{\frac{x(y + 2x) + 3y(y + 2x)}{x^2y^2}}$
>
> $= \frac{\frac{2}{y^2} - \frac{5}{xy} - \frac{3}{x^2}}{\frac{(x + 3y)(y + 2x)}{x^2y^2}}$
>
> $= \frac{\frac{2x^2}{x^2y^2} - \frac{5xy}{x^2y^2} - \frac{3y^2}{x^2y^2}}{\frac{(x + 3y)(y + 2x)}{x^2y^2}}$
>
> $= \frac{\frac{2x^2 - 5xy - 3y^2}{x^2y^2}}{\frac{(x + 3y)(y + 2x)}{x^2y^2}}$
>
> $= \frac{\frac{x(y + 2x) - 3y(y + 2x)}{x^2y^2}}{\frac{(x + 3y)(y + 2x)}{x^2y^2}}$
>
> $= \frac{\frac{(x - 3y)(y + 2x)}{x^2y^2}}{\frac{(x + 3y)(y + 2x)}{x^2y^2}}$
>
> $= \frac{(x - 3y)(y + 2x)(x^2y^2)}{(x + 3y)(y + 2x)(x^2y^2)}$
>
> $= \frac{x - 3y}{x + 3y}$