# Equation Review Part 2

## Solve each of the following equations.

1. $\frac{1}{x} = \frac{2}{x - 3}$
> $= \frac{2}{2x} = \frac{2}{x - 3}$
> 
> $= 2x = x - 3$
> 
> $= x = -3$
2. $\frac{3}{x + 1} - \frac{1}{x - 2} = \frac{1}{x^2 - x - 2}$
> $\frac{3(x - 2)}{(x + 1)(x - 2)} - \frac{x + 1}{(x + 1)(x - 2)} = \frac{1}{x^2 - x - 2}$
> 
> Factors of $-2$ that add up to $-1$ are $\set{1, -2}$<br>
> $\frac{3(x - 2)}{(x + 1)(x - 2)} - \frac{x + 1}{(x + 1)(x - 2)} = \frac{1}{(x + 1)(x - 2)}$
>
> $= \frac{3(x - 2) - (x + 1)}{(x + 1)(x - 2)} = \frac{1}{(x + 1)(x - 2)}$
>
> $= 3(x - 2) - (x + 1) = 1$
>
> $= 3x - 6 - x - 1 = 1$
>
> $= 2x - 7 = 1$
>
> $= 2x = 8$
>
> $x = 4$
3. $\frac{64}{x^2 - 16} + 1 = \frac{2x}{x - 4}$
> $\frac{64}{(x + 4)(x - 4)} + 1 = \frac{2x}{x - 4}$
>
> $\frac{64}{(x + 4)(x - 4)} + \frac{(x + 4)(x - 4)}{(x + 4)(x - 4)} = \frac{2x}{x - 4}$
>
> $= \frac{64 + (x + 4)(x - 4)}{(x + 4)(x - 4)} = \frac{2x}{x - 4}$
> 
> $= \frac{64 + (x + 4)(x - 4)}{(x + 4)} = 2x$
>
> $= 64 + (x + 4)(x - 4) = 2x(x + 4)$
>
> $= x^2 + 48 = 2x^2 + 8x$
>
> $= -(x^2 - 8x + 48) = 0$
>
> Factors of $48$ that add up to $-8$ are $\set{ -4, 12 }$<br>
> $= -(x - 4)(x + 12) = 0$
>
> Split factors<br>
> $= x = \set{ 4, -12 }$
4. $\frac{-15}{4x + 1} = x - 4$
> $= -15 = (x - 4)(4x + 1)$
>
> $= -15 = 4x^2 + x - 16x - 4$
>
> $= 0 = 4x^2 - 15x + 11$
>
> Factors of $44$ that add up to $-15$ are $\set{ -4, 11 }$<br>
> $= 0 = 4x^2  - 4x - 11x + 11$
>
> $= 0 = 4x(x - 1) - 11(x - 1)$
>
> $= 0 = (4x - 11)(x - 1)$
>
> Split factors<br>
> $= x = \set{\frac{11}{4}, 1}$
5. $\sqrt{x - 10} - 4 = 0$
> $= \sqrt{x - 10} = 4$
>
> $= x - 10 = 16$
>
> $= x = 26$
6. $\sqrt[3]{2x + 1} = 3$
> $= 2x + 1 = 27$
> 
> $= 2x = 26$
> 
> $= x = 13$
7. $\sqrt{13x - 29} - x = 1$
> $= \sqrt{13x - 29} = 1 + x$
> 
> $= 13x - 29 = (1 + x)(1 + x)$
> 
> $= 13x - 29 = x^2 + 2x + 1$
> 
> $= x² - 11 + 30 = 0$
> 
> Factors of $30$ that add up to $-11$ are $\set{ -5, -6 }$<br>
> $= (x - 5)(x - 6) = 0$
> 
> Split factors<br>
> $= x = \set{ 5, 6 }$
8. $\sqrt{2x + 5} + 3 = 0$
> $= \sqrt{2x + 5} = -3$
>
> $= 2x + 5 = 9$
>
> $= 2x = 4$
>
> $= x = +2$
9. $|3x + 2| = 7$
> Split into two equations<br>
> $= 3x + 2 = 7$
> > $= 3x = 5$
> >
> > $= x = \frac{5}{3}$
>
> $= -3x - 2 = 7$
> > $= -3x = 9$
> >
> > $= x = -3$
>
> $= x = { \frac{5}{3}, -3 }$
10.   $|x^2 + 3x - 2| = 2$
> Split into two equations<br>
> $= x² + 3x - 2 = 2$
> > $= x² + 3x - 4 = 0$
> >
> > Factors of $-4$ that add up to $3$ are $\set{ 4, -1 }$<br>
> > $= (x + 4)(x - 1) = 0$
> >
> > Split factors<br>
> > $= x = \set{ -4, 1 }$
>
> $= -x² - 3x + 2 = 2$
> > $= x² + 3x = 0$
> >
> > $= x(x + 3) = 0$
> >
> > Split factors<br>
> > $= x = \set{ 0, -3 }$
>
> $= x = \set{ -4, 1, 0, -3 }$

## Solve for the specified variable.

11. $F = \frac{mv^2}{R}$ for $R$
> $= \frac{1}{F} = \frac{R}{mv^2}$
> 
> $= \frac{mv^2}{F} = R$
12. $F = \frac{mv^2}{R} for $v$
> $= FR = mv^2$
> 
> $= \frac{FR}{m} = v^2$
> 
> $= \pm \sqrt{\frac{FR}{m}} = v$
>
> $= \pm \frac{\sqrt{FR}}{\sqrt{m}} = v$
13. $\frac{1}{2x} + \frac{2}{y} = \frac{1}{z}$ for $y$
> $= \frac{y}{2xy} + \frac{4x}{2xy} = \frac{1}{z}$
>
> $= z(y + 4x) = 2xy$
>
> $= 4xz + yz = 2xy$
>
> $= yz = 2xy - 4xz$
>
> $= yz - 2xy = -4xz$
>
> $= y(z - 2x) = -4xz$
>
> $= y = \frac{-4xz}{z - 2x}$
14. $\frac{3x - y}{4x} = \frac{2 - xy}{4}$ for $y$
> $= 3x - y = x(2 - xy)$
>
> $= 3x - y = 2x - x^2y$
>
> $= -y + x^2y = -x$
>
> $= y(x^2 - 1) = -x$
>
> $= y = -\frac{x}{x² - 1}$