# Operations on Functions

# Find each for the functions given.

1. $f(x) = 5 - x$ $g(x) = x^2 - 25$

- $(f + g)(x)$
> $= f(x) + g(x)$
>
> $= 5 - x + x^2 - 25$
>
> $= x^2 - x - 20$
>
> Factors of $-20$ that add up to $-1$ are $\set{ 4, -5 }$<br>
> $= (x + 4)(x - 5)$
- $(f - g)(x)$
> $= f(x) - g(x)$
>
> $= 5 - x - x^2 + 25$
>
> $= -x^2 - x + 30$
>
> $= -(x^2 + x - 30)$
>
> Factors of $-30$ that add up to $1$ are $\set{ 6, -5 }$<br>
> $= -(x + 6)(x - 5)$
- $(fg)(x)$
> $= f(x) * g(x)$
>
> $= (5 - x)(x^2 - 25)$
>
> $= 5x^2 - 125 - x^3 + 25x$
>
> $= -x^3 + 5x^2 + 25x - 125$
>
> $= x^3 - 5x^2 - 25x + 125$
>
> $= x(x^2 - 25) - 5(x^2 - 125)$
>
> $= (x - 5)(x^2 - 25)$
>
> $= (x - 5)(x + 5)(x - 5)$
>
> $= (x - 5)^2(x + 5)$
- $\frac{g}{f}(x)$
> $= \frac{g(x)}{f(x)}$
> 
> $= \frac{x^2 - 25}{5 - x}$
> 
> $= \frac{(x + 5)(x - 5)}{5 - x}$
> 
> $= -\frac{(x + 5)(x - 5)}{x - 5}$
> 
> = $-(x + 5)$
> 
> = $-x - 5$
- $f(g(x))$
> $= 5 - g(x)$
> 
> $= 5 - x^2 + 25$
> 
> $= -x^2 + 30$
- $g(f(x))$
> $= f(x)^2 - 25$
>
> $= (5 - x)^2 - 25$
>
> $= (5 - x)(5 - x) - 25$
>
> $= 25 - 5x - 5x + x^2 - 25$
>
> $= x^2 - 10x$
>
> $= x(x - 10)$


2. $f(x) = \frac{x}{x + 3}$, $g(x) = \frac{5}{x^2 - 9}$

- $(f - g)(x)$
> $= f(x) - g(x)$
>
> $= \frac{x}{x + 3} - \frac{5}{x^2 - 9}$
>
> $= \frac{x}{x + 3} - \frac{5}{(x + 3)(x - 3)}$
>
> $= \frac{x(x - 3)}{(x + 3)(x - 3)} - \frac{5}{(x + 3)(x - 3)}$
>
> $= \frac{x(x - 3) - 5}{(x + 3)(x - 3)}$
>
> $= \frac{x^2 - 3x - 5}{(x + 3)(x - 3)}$
- $(\frac{g}{f})(x)$
> $= \frac{g(x)}{f(x)}$
> 
> $= \frac{\frac{5}{x^2 - 9}}{\frac{x}{x + 3}}$
>
> $= \frac{5(x + 3)}{x(x^2 - 9)}$
>
> $= \frac{5(x + 3)}{x(x + 3)(x - 3)}$
>
> $= \frac{5}{x(x - 3)}$
- $(gf)(5)$
> $= g(5) \cdot f(5)$
>
> $= \frac{5}{5^2 - 9} \cdot \frac{5}{5 + 3}$
>
> $= \frac{5}{25 - 9} \cdot \frac{5}{8}$
>
> $= \frac{5}{16} \cdot \frac{5}{8}$
>
> $= \frac{25}{128}$
- $f(g(x))$
> $= \frac{g(x)}{g(x) + 3}$
> 
> $= \frac{\frac{5}{x^2 - 9}}{\frac{5}{x^2 - 9} + 3}$
>
> $= \frac{\frac{5}{(x + 3)(x - 3)}}{\frac{5}{(x + 3)(x - 3)} + 3}$
>
> $= \frac{\frac{5}{(x + 3)(x - 3)}}{\frac{5}{(x + 3)(x - 3)} + \frac{3(x + 3)(x - 3)}{(x + 3)(x - 3)}}$
> 
> $= \frac{\frac{5}{(x + 3)(x - 3)}}{\frac{5 + 3(x + 3)(x - 3)}{(x + 3)(x - 3)}}$
>
> $= \frac{5(x + 3)(x - 3)}{(5 + 3(x + 3)(x - 3))(x + 3)(x - 3)}$
>
> $= \frac{5}{5 + 3(x + 3)(x - 3)}$
>
> $= \frac{5}{3x^2 - 27}$
> 
> $= \frac{5}{3x^2 - 22}$
- $f(f(x))$
> $= \frac{f(x)}{f(x) + 3}$
>
> $= \frac{\frac{x}{x + 3}}{\frac{x}{x + 3} + 3}$
>
> $= \frac{x}{(x + 3)(\frac{x}{x + 3} + 3)}$
>
> $= \frac{x}{(x + 3)(\frac{x}{x + 3} + \frac{3(x + 3)}{x + 3})}$
>
> $= \frac{x}{(x + 3)\frac{x + 3(x + 3)}{x + 3}}$
>
> $= \frac{x}{x + 3(x + 3)}$
>
> $= \frac{x}{4x + 9}$

3. $f(x) = \sqrt[3]{x - 1}$, $g(x) = x^3 + 1$

- $f(g(x))$
> $= \sqrt[3]{g(x) - 1}$
> 
> $= \sqrt[3]{x^3 + 1 - 1}$
> 
> $= \sqrt[3]{x^3}$
> 
> $= x$
- $g(f(x))$
> $= f(x)^3 + 1$
> 
> $= \sqrt[3]{x - 1}^3 + 1$
> 
> $= (x - 1) + 1$
> 
> $= x$
- $f(g(0))$
> $= \sqrt[3]{g(0) - 1}$
>
> $= \sqrt[3]{(0^3 + 1) - 1}$
>
> $= \sqrt[3]{0 + 1 - 1}$
>
> $= \sqrt[3]{0}$
>
> $= 0$

4. $f(x) = \frac{1}{3}x - 3$, $g(x) = 3x + 1$

- $f(g(x))$
> $= \frac{1}{3}(g(x)) - 3$
> 
> $= \frac{1}{3}(3x + 1) - 3$
> 
> $= \frac{3x + 1}{3} - 3$
> 
> $= \frac{3x + 1}{3} - \frac{9}{3}$
> 
> $= \frac{3x - 8}{3}$
- $g(f(x))$
> $= 3(f(x)) + 1$
>
> $= 3(\frac{x}{3} - 3) + 1$
>
> $= x - 9 + 1$
>
> $= x - 8$
- $(g - f)(x)$
> $= g(x) - f(x)$
>
> $\frac{9x}{3} + 1 - \frac{x}{3} + 3$
>
> $\frac{8x}{3} + 4$
>
> $\frac{8x}{3} + \frac{12}{3}$
>
> $\frac{8x + 12}{3}$
>
> $\frac{4(2x + 3)}{3}$

5. Analyze the graph at the right.

- $(f - g)(1)$
> $= f(1) - g(1)$
> 
> $= 4 - 7$
>
> $= -3$
- $(f + g)(0)$
> $= f(0) + g(0)$
>
> $= 3 + 7$
>
> $= 10$
- $f(g(-8))$
> $= f(1)$
>
> $= 4$
- $g(f(1))$
> $= g(4)$
>
> $= 7$
- $f(g(1))$
> $= f(7)$
>
> $= 10$
- $f(f(-1))$
> $= f(2)$
>
> $= 5$
- Where is $(f - g)(x) = 0$?
> $= f(x) - g(x) = 0$
>
> $= f(x) = g(x)$
>
> $= x = \set{ -7, 3 }$
- Where is $(f - g)(x) \gt 0$?
> $= f(x) \gt g(x)$
>
> $= [-9, -7] \cup [3, 7]$
- Where is $f(x) \le g(x)$?
> $= [-7, 3]$

6. Analyze the following graph.

- $f(0)$
- $f(-2)$
- Where does $f(x) = -2$?
- Where does $f(x) = 0$?
- For what x-values is $f(x) > 0$?
- For what x-values is $f(x) <= 0$?
- State the domain:
- Range:
- Zeroes:
- Where is $f$ increasing?
- Where is $f$ decreasing?

7. Find the domain of each of the following

- $f(x) = \frac{4}{x - 1}$
> $x \in \R$ where $x \ne 1$
>
> $\lparen -\infty, 1\rparen \cup \lparen 1, +\infty\rparen$
- $f(x) = 2x^2 + 3$
> $x \in \R$
>
> $(-\infty, +\infty)$
- $f(x) = \frac{1}{x + 2}$
> $x \in \R$ where $x \ne -2$
>
> $\lparen -\infty, -2\rparen \cup \lparen -2, +\infty\rparen$
- $f(x) = \frac{1}{x^2 - 3}$
> $x \in \R$ where $x \ne \pm \sqrt{3}$
>
> $(-\infty, -\sqrt{3}) \cup (-\sqrt{3}, \sqrt{3}) \cup (\sqrt{3}, +\infty)$
- $f(x) = \sqrt{x - 3}$
> $x \in R$ where $x \ge 3$
>
> $\lbrack 3, +\infty\rparen$
- $f(x) = -x + 5$
> $x \in R$
>
> $(-\infty, +\infty)$