# Topic: Algebraic Expressions Review

## Simplify each of the following. Leave answers in factored form.

1. $\frac{x + 3}{x² - 4} \cdot \frac{x³ - 8}{x² - x - 12}$
> $= \frac{(x + 3)(x³ - 8)}{(x² - 4)(x² - x - 12)}$
> 
> $= \frac{(x + 3)(x³ - 8)}{(x² - 4)(x + 3)(x - 4)}$
> 
> Difference of squares: $a² - b² = (a + b)(a - b)$<br>
> $= \frac{(x + 3)(x³ - 8)}{(x + 2)(x - 2)(x + 3)(x - 4)}$
> 
> Difference of cubes: $a³ − b³ = (a − b)(a² + ab + b²)$<br>
> $= \frac{(x + 3)(x - 2)(x² + 2x + 4)}{(x + 2)(x - 2)(x + 3)(x - 4)}$
> 
> $= \frac{x² + 2x + 4}{(x + 2)(x - 4)}$

2. $\frac{\frac{x² - 4}{2x² - 5x + 2}}{\frac{2x² - 3x - 2}{4x² - 1}}$
> $= \frac{(x² - 4)(4x² - 1)}{(2x² - 5x + 2)(2x² - 3x - 2)}$
> 
> Difference of squares: $a² - b² = (a + b)(a - b)$<br>
> $= \frac{(x² - 4)(2x - 1)(2x + 1)}{(x - 2)(2x + 1)(2x² - 5x + 2)}$
> 
> $= \frac{(x² - 4)(2x - 1)}{(x - 2)(2x² - 5x + 2)}$
> 
> $= \frac{(x² - 4)(2x - 1)}{(x - 2)(2x² - 4x - x + 2)}$
> 
> $= \frac{(x² - 4)(2x - 1)}{(x - 2)(x(2x - 1) - 2(2x - 1))}$
> 
> $= \frac{(x² - 4)(2x - 1)}{(x - 2)(x - 2)(2x - 1)}$
> 
> Difference of squares: $a² - b² = (a + b)(a - b)$<br>
> $= \frac{(x + 2)(x - 2)(2x - 1)}{(x - 2)(x - 2)(2x - 1)}$
> 
> $= \frac{x + 2}{x - 2}$

3. $\frac{3}{2xy} + \frac{7}{6x²}$
> $= \frac{3x(3)}{3x(2xy)} + \frac{y(7)}{y(6x²)}$
> 
> $= \frac{9x}{6x²y} + \frac{7y}{6x²y}$
> 
> $= \frac{9x + 7x}{6x²y}$

4. $\frac{x - 3}{x + 4} - \frac{x}{x - 2}$
> $= \frac{(x - 2)(x - 3)}{(x - 2)(x + 4)} - \frac{x(x + 4)}{(x - 2)(x + 4)}$
> 
> $= \frac{(x - 2)(x - 3) - x(x + 4)}{(x - 2)(x + 4)}$
> 
> $= \frac{(x² - 5x + 6) - (x² + 4x)}{(x - 2)(x + 4)}$
>
> $= \frac{(x² - 5x + 6) - (x² + 4x)}{(x - 2)(x + 4)}$
> 
> $= \frac{-9x + 6}{(x - 2)(x + 4)}$
> 
> $= \frac{3(-3x + 2)}{(x - 2)(x + 4)}$

5. $\frac{4x}{x² - 4} + \frac{2}{x² - 5x + 6}$
> Difference of squares:<br>
> $= \frac{4x}{(x + 2)(x - 2)} + \frac{2}{x² - 5x + 6}$
>
> Factors of $6$ that add up to $-5$ are $\set{-2, -3}$<br>
> $= \frac{4x}{(x + 2)(x - 2)} + \frac{2}{(x - 2)(x - 3)}$
>
> $= \frac{4x(x - 3)}{(x + 2)(x - 2)(x - 3)} + \frac{2(x + 2)}{(x + 2)(x - 2)(x - 3)}$
>
> $= \frac{4x(x - 3) + 2(x + 2)}{(x + 2)(x - 2)(x - 3)}$
>
> $= \frac{4x^2 - 12x + 2x + 4}{(x + 2)(x - 2)(x - 3)}$
>
> $= \frac{4x^2 - 10x + 4}{(x + 2)(x - 2)(x - 3)}$
>
> $= \frac{2(2x^2 - 5x + 2)}{(x + 2)(x - 2)(x - 3)}$
>
> Factors of $4$ ($2 \cdot 2$) that add up to $-5$ are $\set{-1, -4}$<br>
> $= \frac{2(x - 2)(2x - 1)}{(x + 2)(x - 2)(x - 3)}$
>
> $= \frac{2(2x - 1)}{(x + 2)(x - 3)}$

6. `((x² / (x - 3))) + (9 / (3 - x))`
> ```rs
> // if `a - b = c` then `b - a = -c`
> = ((x² / (x - 3))) - (9 / (x - 3))
> = (x² - 9) / (x - 3)
> // Difference of squares: a² - b² = (a + b)(a - b)
> = (x + 3)(x - 3) / (x - 3)
> = (x + 3)
> ```

1. `((1 / 2) + (1 / x)) / ((x + 3) / 4)`
> ```rs
> = ((x / 2x) + (2 / 2x)) / ((x + 3) / 4)
> = ((x + 2) / 2x) / ((x + 3) / 4)
> = 4(x + 2) / 2x(x + 3)
> = 2(x + 2) / x(x + 3)
> ```

1. `((x / (x² - 4)) + (3 / (x - 2))) / ((5 / (x + 2)) + (4 / (x - 2)))`
> ```rs
> = ((x / (x² - 4)) + (3 / (x - 2))) / ((5(x - 2) / (x + 2)(x - 2)) + (4(x + 2) / (x - 2)(x + 2)))
> = ((x / (x² - 4)) + (3 / (x - 2))) / (5(x - 2) + 4(x + 2) / (x - 2)(x + 2))
> = ((x / (x² - 4)) + (3 / (x - 2))) / ((5x - 10 + 4x + 8) / (x - 2)(x + 2))
> = ((x / (x² - 4)) + (3 / (x - 2))) / ((9x - 2) / (x - 2)(x + 2))
> // Difference of squares: a² - b² = (a + b)(a - b)
> = ((x / (x + 2)(x - 2)) + (3 / (x - 2))) / ((9x - 2) / (x - 2)(x + 2))
> = ((x / (x + 2)(x - 2)) + (3(x + 2) / (x + 2)(x - 2))) / ((9x - 2) / (x - 2)(x + 2))
> = ((x + 3(x + 2)) / (x + 2)(x - 2)) / ((9x - 2) / (x - 2)(x + 2))
> = ((4x + 6) / (x + 2)(x - 2)) / ((9x - 2) / (x - 2)(x + 2))
> = (2(2x + 3) / (x + 2)(x - 2)) / ((9x - 2) / (x - 2)(x + 2))
> = (2(2x + 3) / (x + 2)(x - 2))(x - 2)(x + 2) / (9x - 2)
> = 2(2x + 3) / (9x - 2)
> ```
