# Topic: Equation Review

## Solve the following equations for x.

1. $(3x - 2) - \frac{1}{4}(x - 5) = 10$
> Turn multiplication with fraction into division<br>
> $(3x - 2) - \frac{x - 5}{4} = 10$
> 
> Give $(3x - 2)$ a denominator of $4$ by multiplying both sides<br>
> $\frac{4(3x - 2)}{4} - \frac{x - 5}{4} = 10$
> 
> Join fractions<br>
> $\frac{4(3x - 2) - (x - 5)}{4} = 10$
> 
> Factor out $-1$ from $-(x - 5)$<br>
> $\frac{4(3x - 2) + -x + 5}{4} = 10$
> 
> Distribute constant term $4$<br>
> $\frac{12x - 8 + -x + 5}{4} = 10$
> 
> Join terms<br>
> $\frac{11x - 3}{4} = 10$
> 
> Multiply both sides by $4$<br>
> $11x - 3 = 40$
> 
> Add $3$ to both sides<br>
> $11x = 43$
> 
> Divide both sides by $11$<br>
> $x = \frac{43}{11}$

2. $5x² + 3x - 2 = 0$
> $5 \cdot -2 = -10$, factors of $-10$ that add up to $3$ are $\set{ 5, -2 }$<br>
> $= 5x² + 5x - 2x - 2 = 0$
> 
> Rearrange<br>
> $= 5x - 2 + 5x² - 2x = 0$
> 
> Factor by grouping<br>
> $= (5x - 2) + (5x² - 2x) = 0$
> 
> $= (5x - 2) + x(5x - 2) = 0$
> 
> $= (x + 1)(5x - 2) = 0$
> 
> Split factors<br>
> $= x = \set{ -1, \frac{2}{5} }$

3. $3x² - 48 = 0$
> Factor out $3$<br>
> $= 3(x² - 16) = 0$
> 
> Difference of squares: $a² - b² = (a + b)(a - b)$<br>
> $= 3(x + 4)(x - 4) = 0$
> 
> Divide both sides by $3$<br>
> $= (x + 4)(x - 4) = 0$
> 
> Split factors<br>
> $= x = \set{ 4, -4 }$

4. $x² + 4x + 2 = 0`$
> Add $2$ to both sides<br>
> $= x² + 4x + 4 = 2$
> 
> Factors of $4$ that add to $4$ are $\set{ 2, 2 }$<br>
> $= (x + 2)(x + 2) = 2$
> 
> $= (x + 2)² = 2$
> 
> $= x + 2 = \pm \sqrt{2}$
> 
> $= x = \pm \sqrt{2} - 2$

5. $9x² - 20 = 0$
> Add $20$ to both sides<br>
> $= 9x² = 20$
> 
> $= x² = \frac{20}{9}$
> 
> $= x = \pm \sqrt{\frac{20}{9}}$
> 
> $= x = \pm \frac{\sqrt{20}}{\sqrt{9}}$
> 
> $= x = \pm \frac{\sqrt{20}}{3}$
> 
> $= x = \pm \frac{2 \sqrt{5}}{3}$

6. $2x³ - x² - 18x + 9 = 0`$
> Factor by grouping<br>
> $= (2x³ - x²) + (-18x + 9) = 0$
> 
> $= x²(2x - 1) - 9(2x - 1) = 0$
> 
> $= (x² - 9)(2x - 1) = 0$
> 
> Difference of squares: $a² - b² = (a + b)(a - b)$<br>
> $= (x + 3)(x - 3)(2x - 1) = 0$
> 
> Split factors<br>
> $= x = \set{ \pm 3, \pm \frac{1}{2} }$

7. $x^4 = 2x² - 1$
> $x^4 - 2x² + 1 = 0$
> 
> Let $y = x²$<br>
> $= y² - 2y + 1 = 0$
> 
> Factors of $1$ that add up to $-2$ are $\set{ -1, -1 }$<br>
> $(y - 1)(y - 1) = 0$
> 
> $(y - 1)² = 0$
> 
> $(x² - 1)² = 0$
> 
> Difference of squares: $a² - b² = (a + b)(a - b)$<br>
> $(x + 1)²(x - 1)² = 0$
> 
> $(x + 1)(x + 1)(x - 1)(x - 1) = 0$
> 
> Split factors<br>
> $= x = \set{ 1, -1 }$

## Solve for the specified variable

8. $A = \frac{1}{2}(bh)$ for $h$
> $A = \frac{1}{2}(bh)$
> 
> $2A = bh$
> 
> $\frac{2A}{b} = h$

9. $ax + by = ab$ for $b$
> $= ax + by - ba = 0$
> 
> $= ax + b(y - a) = 0$
> 
> $b(y - a) = -ax$
> 
> $b = -\frac{ax}{y - a}$

