# Topic: Equation Review Part 2

## Solve the following equations for x. State any values not in the domain of x.

1. $\frac{6}{x} + \frac{8}{x + 5} = 3$
> Get a common denominator by multiplying both parts<br>
> $= \frac{6(x + 5)}{x(x + 5)} + \frac{8x}{x(x + 5)} = 3$
> 
> Combine like terms<br>
> $= \frac{6(x + 5) + 8x}{x(x + 5)} = 3$
> 
> Move $x(x + 5)$<br>
> $= 6(x + 5) + 8x = 3x(x + 5)$
> 
> Multiply terms<br>
> $= 6x + 30 + 8x = 3x² + 15x$
> 
> $= 14x + 30 = 3x² + 15x$
> 
> $= -3x² - 15x + 14x + 30 = 0$
> 
> $= -3x² - x + 30 = 0$
> 
> Factor out $-1$<br>
> $= -(3x² + x - 30) = 0$
> 
> Products of $-90$ that add to $1$ are $\set{ -9, 10 }$<br>
> $= -(10(x - 3) + 3x(x - 3)) = 0$
> 
> $= (3x + 10)(x - 3) = 0$
> 
> Split factors<br>
> $= x = \set{ -\frac{10}{3}, 3 }$
> 
> $= x \ne \set{ 0, -5 }$

2. $\frac{x + 2}{x - 3} = \frac{30}{x^2 - 9} + \frac{1}{x + 3}$
> Difference of squares: $a² - b² = (a + b)(a - b)$<br>
> $= \frac{x + 2}{x - 3} = \frac{30}{(x + 3)(x - 3)} + \frac{1}{x + 3}$
> 
> Multiply by $(x + 3)(x - 3)$<br>
> $= \frac{(x + 2)(x + 3)(x - 3)}{x - 3} = \frac{30(x + 3)(x - 3)}{(x + 3)(x - 3)} + \frac{(x + 3)(x - 3)}{x + 3}$
> 
> $= (x + 2)(x + 3) = x + 27$
> 
> $= x² + 5x + 6 = x + 27$
> 
> $= x² + 4x - 21 = 0$
> 
> Products of $-21$ that add to $4$ are $\set{ 7, -3 }$<br>
> $= (x + 7)(x - 3) = 0$
> 
> Split factors<br>
> $= x = -7$ (3 is removed as a root)
> 
> $= x ≠ { +3, -3 }$
> ```

## Solve the following equations for x.

3. $\sqrt{x + 3} = 5$
> $= x + 3 = 25$
> 
> $= x = 22$

4. $\sqrt{4 - x} = 2 - x$
> $= 4 - x = (2 - x)²$
> 
> $= 4 - x = (2 - x)(2 - x)$
> 
> $= 4 - x = 4 - 2x - 2x + x²$
> 
> $= 4 - x = x² - 4x + 4 $
> 
> $= x² - 5x = 0$
> 
> $= x(x - 5) = 0$
> 
> $5$ is removed as a root as $\sqrt{4 - 5} = i$, not in $\R$<br>
> $= x = 0$

5. $\sqrt[3]{3x - 1} + 4 = 0$
> $= \sqrt[3]{3x - 1} = -4$
> 
> $= 3x - 1 = -64$
> 
> $= 3x = -63$
> 
> $= x = -21$

6. $|2x + 3| = 5$
> Split into 2 equations<br>
> $= 2x + 3 = 5$
> > $= 2x = 2$
> >
> > $= x = 1$
> 
> $= -2x - 3 = 5$
> > $= -2x = 8$
> >
> > $= x = -4$
>
> $= x = { 1, -4 }$

## Solve for the specified variable.

7. $\frac{1}{R} = \frac{1}{R_1} + \frac{1}{R_2}$
> $=\frac{1}{R} = \frac{R_2}{R_1R_2} + \frac{R_1}{R_1R_2}$
> 
> $= \frac{1}{R} = \frac{R_1 + R_2}{R₁R₂}$
> 
> Assuming $R_1 \ne 0$ and $R_2 \ne 0$<br>
> $= R = \frac{R_1R_2}{R_1 + R_2}$
