# Topic: Factoring Review

## Multiply the following polynomials.

1. $(x + 5)(2x - 3)$
> $= 2x² + 7x - 15$
2. $(2x - 5)²$
> $= (2x - 5)(2x - 5)$
> 
> $= 4x² - 20x + 25$
3. $(x² - 2x + 1)(x + 3)$
> $= x³ - 2x² + x + 3x² - 6x + 3$
> $= x³ + x² - 5x + 3$

## Factor each polynomial completely.

4. $x² - 6x + 8$
> $= (x - 4)(x - 2)$
5. $27x² - 48$
> $= 3(9x² - 16)$
> 
> $= 3(3x - 4)(3x + 4)$
6. $-15x² - 5x$
> $= -5x(3x + 1)$
7. $4x² + 12x + 9$
> $= (2x + 3)²$
8. $2x² - 3x - 9$
> $= (2x + 3)(x - 3)$
9. $x³ - 4x² + 2x - 8$
> $= (x³ - 4x²) + (2x - 8)$
> 
> $= x²(x - 4) + 2(x - 4)$
> 
> $= (x - 4)(x² + 2)$
10. $8x³ - 10x² - 3x$
> $= x(8x² - 10x - 3)$
> 
> $= x(8x² - 12x + 2x - 3)$
> 
> $= x(2x(4x + 1) - 3(4x + 1))$
> 
> $= x(2x - 3)(4x + 1)$
11. $x³ - 8$
> Difference of cubes: $a³ - b³ = (a - b)(a² + ab + b²)$<br>
> $= (x - 2)(x² + 2x + 4)$
12. $x⁴ - 81$
> Difference of squares: $a² - b² = (a + b)(a - b)$<br>
> $= (x² + 9)(x² - 9)$
> 
> $= (x² + 9)(x + 3)(x - 3)$